thys/Circus/Denotational_Semantics.thy
@@ -1,119 +1,405 @@
-(*  Title:       Isabelle/Circus
-    Author:      Abderrahmane Feliachi, Burkhart Wolff, Marie-Claude Gaudel
-                 Univ. Paris-Sud / LRI
-    Maintainer:  Abderrahmane Feliachi
-*)
+header {* Denotational semantics of Circus actions *}
 
 theory Denotational_Semantics 
-imports Circus_Actions
+imports Circus_Actions Var_list
 begin
 
-subsection {* Circus Denotational semantics of actions \label{Denotational}*}
-
-text {* In this subsection, we introduce the definitions of Circus actions denotational semantics.
+text {* In this section, we introduce the definitions of Circus actions denotational semantics.
 We provide the proof of well-formedness of every action. We also provide proofs concerning 
 the monotonicity of operators over actions.*}
 
-subsubsection {* Stop *}
-
-definition Stop :: "('\<theta>::ev_eq,'\<sigma>) action"
-where "Stop \<equiv> action_of (R (true \<turnstile> \<lambda>(A, A'). tr A' = tr A \<and> wait A'))"
-
-lemma Stop_is_action:
-"(R (true \<turnstile> \<lambda>(A, A'). tr A' = tr A \<and> wait A')) : action"
-apply (simp add: action_def)
-apply (rule rd_is_CSP)
-by auto
-
-lemmas Stop_is_CSP = Stop_is_action[simplified action_def]
-
-lemma relation_of_Stop:
-"relation_of Stop = (R (true \<turnstile> \<lambda>(A, A'). tr A' = tr A \<and> wait A'))"
-by (simp add: Stop_def action_of_inverse Stop_is_action)
-
-subsubsection {* Skip *}
+subsection {* Skip *}
 
 definition Skip :: "('\<theta>::ev_eq,'\<sigma>) action" where
 "Skip \<equiv> action_of 
                   (R (true \<turnstile> \<lambda>(A, A'). tr A' = tr A \<and> \<not>wait A' \<and> more A = more A'))"
 
 lemma Skip_is_action: 
-"(R (true \<turnstile> \<lambda>(A, A'). tr A' = tr A \<and> \<not>wait A' \<and> more A = more A')) : action"
-apply (simp add: action_def)
+"(R (true \<turnstile> \<lambda>(A, A'). tr A' = tr A \<and> \<not>wait A' \<and> more A = more A')) \<in> {p. is_CSP_process p}"
+apply (simp)
 apply (rule rd_is_CSP)
 by auto
 
-lemmas Skip_is_CSP = Skip_is_action[simplified action_def]
+lemmas Skip_is_CSP = Skip_is_action[simplified]
 
 lemma relation_of_Skip: 
 "relation_of Skip = 
                   (R (true \<turnstile> \<lambda>(A, A'). tr A' = tr A \<and> \<not>wait A' \<and> more A = more A'))"
-by (simp add: Skip_def action_of_inverse Skip_is_action)
+by (simp add: Skip_def action_of_inverse Skip_is_CSP)
 
-subsubsection {* Chaos *}
+definition CSP3::"(('\<theta>::ev_eq,'\<sigma>) alphabet_rp) Healthiness_condition"
+where "CSP3 (P)  \<equiv>  relation_of Skip ;; P"
+
+definition CSP4::"(('\<theta>::ev_eq,'\<sigma>) alphabet_rp) Healthiness_condition"
+where "CSP4 (P)  \<equiv>  P ;; relation_of Skip"
+
+lemma Skip_is_CSP3: "(relation_of Skip) is CSP3 healthy"
+apply (auto simp: relation_of_Skip rp_defs design_defs fun_eq_iff CSP3_def)
+apply (split cond_splits, simp_all)+
+apply (rule_tac b=b in comp_intro)
+apply (split cond_splits, simp_all)+
+apply (rule_tac b=b in comp_intro)
+apply (split cond_splits, simp_all)+
+prefer 3
+apply (split cond_splits, simp_all)+
+apply (auto simp add: prefixeq_def)
+done
+
+lemma Skip_is_CSP4: "(relation_of Skip) is CSP4 healthy"
+apply (auto simp: relation_of_Skip rp_defs design_defs fun_eq_iff CSP4_def)
+apply (split cond_splits, simp_all)+
+apply (rule_tac b=b in comp_intro)
+apply (split cond_splits, simp_all)+
+apply (rule_tac b=b in comp_intro)
+apply (split cond_splits, simp_all)+
+prefer 3
+apply (split cond_splits, simp_all)+
+apply (auto simp add: prefixeq_def)
+done
+
+
+lemma Skip_comp_absorb: "(relation_of Skip ;; relation_of Skip) = relation_of Skip"
+apply (auto simp: relation_of_Skip fun_eq_iff rp_defs true_def design_defs)
+apply (clarsimp split: cond_splits)+
+apply (case_tac "ok aa", simp_all)
+apply (erule disjE)+
+apply (clarsimp simp: prefixeq_def)
+apply (clarsimp simp: prefixeq_def)
+apply (erule disjE)+
+apply (clarsimp simp: prefixeq_def)
+apply (clarsimp simp: prefixeq_def)
+apply (erule disjE)+
+apply (clarsimp simp: prefixeq_def)
+apply (clarsimp simp: prefixeq_def)
+apply (case_tac "ok aa", simp_all)
+apply (clarsimp simp: prefixeq_def)
+apply (clarsimp split: cond_splits)+
+apply (rule_tac b=a in comp_intro)
+apply (clarsimp split: cond_splits)+
+apply (rule_tac b=a in comp_intro)
+apply (clarsimp split: cond_splits)+
+done
+
+
+subsection {* Stop *}
+
+definition Stop :: "('\<theta>::ev_eq,'\<sigma>) action"
+where "Stop \<equiv> action_of (R (true \<turnstile> \<lambda>(A, A'). tr A' = tr A \<and> wait A'))"
+
+lemma Stop_is_action:
+"(R (true \<turnstile> \<lambda>(A, A'). tr A' = tr A \<and> wait A')) \<in> {p. is_CSP_process p}"
+apply (simp)
+apply (rule rd_is_CSP)
+by auto
+
+lemmas Stop_is_CSP = Stop_is_action[simplified]
+
+lemma relation_of_Stop:
+"relation_of Stop = (R (true \<turnstile> \<lambda>(A, A'). tr A' = tr A \<and> wait A'))"
+by (simp add: Stop_def action_of_inverse Stop_is_CSP)
+
+
+lemma Stop_is_CSP3: "(relation_of Stop) is CSP3 healthy"
+apply (auto simp: relation_of_Stop relation_of_Skip rp_defs design_defs fun_eq_iff CSP3_def)
+apply (rule_tac b=a in comp_intro)
+apply (split cond_splits, auto)
+apply (split cond_splits)+
+apply (simp_all)
+apply (case_tac "ok aa", simp_all)
+apply (case_tac "tr aa \<le> tr ba", simp_all)
+apply (case_tac "ok ba", simp_all)
+apply (case_tac "tr ba \<le> tr c", simp_all)
+apply (rule disjI1)
+apply (simp add: prefixeq_def)
+apply (erule exE)+
+apply (rule_tac x="zs@zsa" in exI, simp)
+apply (rule disjI1)
+apply (simp add: prefixeq_def)
+apply (erule exE | erule conjE)+
+apply (rule_tac x="zs@zsa" in exI, simp)
+apply (split cond_splits)+
+apply (simp_all add: true_def)
+apply (erule disjE)
+apply (simp add: prefixeq_def)
+apply (erule exE | erule conjE)+
+apply (rule_tac x="zs@zsa" in exI, simp)
+apply (auto simp add: prefixeq_def)
+done
+
+
+lemma Stop_is_CSP4: "(relation_of Stop) is CSP4 healthy"
+apply (auto simp: relation_of_Stop relation_of_Skip rp_defs design_defs fun_eq_iff CSP4_def)
+apply (rule_tac b=b in comp_intro)
+apply (split cond_splits, simp_all)+
+apply (case_tac "ok aa", simp_all)
+apply (case_tac "tr aa \<le> tr ba", simp_all)
+apply (case_tac "ok ba", simp_all)
+apply (case_tac "tr ba \<le> tr c", simp_all)
+apply (rule disjI1)
+apply (simp add: prefixeq_def)
+apply (erule exE)+
+apply (rule_tac x="zs@zsa" in exI, simp)
+apply (rule disjI1)
+apply (simp add: prefixeq_def)
+apply (erule exE | erule conjE)+
+apply (rule_tac x="zs@zsa" in exI, simp)
+apply (split cond_splits)+
+apply (simp_all add: true_def)
+apply (erule disjE)
+apply (simp add: prefixeq_def)
+apply (erule exE | erule conjE)+
+apply (rule_tac x="zs@zsa" in exI, simp)
+apply (auto simp add: prefixeq_def)
+done
+
+subsection {* Chaos *}
 
 definition Chaos :: "('\<theta>::ev_eq,'\<sigma>) action"
 where "Chaos \<equiv> action_of (R(false \<turnstile> true))"
 
-lemma Chaos_is_action: "(R(false \<turnstile> true)) : action"
-apply (simp add: action_def)
+lemma Chaos_is_action: "(R(false \<turnstile> true)) \<in> {p. is_CSP_process p}"
+apply (simp)
 apply (rule rd_is_CSP)
 by auto
 
-lemmas Chaos_is_CSP = Chaos_is_action[simplified action_def]
+lemmas Chaos_is_CSP = Chaos_is_action[simplified]
 
 lemma relation_of_Chaos: "relation_of Chaos = (R(false \<turnstile> true))"
-by (simp add: Chaos_def action_of_inverse Chaos_is_action)
+by (simp add: Chaos_def action_of_inverse Chaos_is_CSP)
 
-subsubsection {* Internal choice *}
+
+subsection {* State update actions*}
+
+definition Pre ::"'\<sigma> relation  \<Rightarrow> '\<sigma> predicate"
+where "Pre sc \<equiv> \<lambda>A. \<exists> A'. sc (A, A')"
+
+
+definition state_update_before :: "'\<sigma> relation \<Rightarrow> ('\<theta>::ev_eq,'\<sigma>) action \<Rightarrow> ('\<theta>,'\<sigma>) action"
+where "state_update_before sc Ac = action_of(R ((\<lambda>(A, A'). (Pre sc) (more A)) \<turnstile> 
+                      (\<lambda>(A, A'). sc (more A, more A') & \<not>wait A' & tr A = tr A')) ;; relation_of Ac)"
+
+lemma state_update_before_is_action: 
+"(R ((\<lambda>(A, A'). (Pre sc) (more A)) \<turnstile> 
+                               (\<lambda>(A, A').sc (more A, more A') & \<not>wait A' & tr A = tr A')) ;; relation_of Ac) \<in> {p. is_CSP_process p}"
+apply (simp)
+apply (rule seq_CSP)
+apply (rule rd_is_CSP1)
+apply (auto simp: R_idem2 Healthy_def relation_of_CSP)
+done
+
+lemmas state_update_before_is_CSP = state_update_before_is_action[simplified]
+
+lemma relation_of_state_update_before:
+"relation_of (state_update_before sc Ac) = (R ((\<lambda>(A, A'). (Pre sc) (more A)) \<turnstile> 
+                               (\<lambda>(A, A'). sc (more A, more A') & \<not>wait A' & tr A = tr A')) ;; relation_of Ac)"
+by (simp add: state_update_before_def action_of_inverse state_update_before_is_CSP)
+
+lemma mono_state_update_before: "mono (state_update_before sc)"
+by (auto simp: mono_def less_eq_action ref_def relation_of_state_update_before design_defs rp_defs fun_eq_iff 
+            split: cond_splits dest: relation_of_spec_f_f[simplified] 
+                                     relation_of_spec_t_f[simplified])
+
+lemma state_update_before_is_CSP3: "relation_of (state_update_before sc Ac) is CSP3 healthy"
+apply (auto simp: relation_of_state_update_before relation_of_Skip rp_defs design_defs fun_eq_iff CSP3_def)
+apply (rule_tac b=aa in comp_intro)
+apply (split cond_splits, auto)
+apply (split cond_splits, simp_all)+
+apply (rule_tac b=bb in comp_intro)
+apply (split cond_splits, simp_all)+
+apply (case_tac "ok aa", simp_all)
+apply (case_tac "tr aa \<le> tr ab", simp_all)
+apply (case_tac "ok ab", simp_all)
+apply (case_tac "tr ab \<le> tr bb", simp_all)
+apply (rule disjI1)
+apply (simp add: prefixeq_def)
+apply (erule exE)+
+apply (rule_tac x="zs@zsa" in exI, simp)
+apply (rule_tac b=bb in comp_intro)
+apply (split cond_splits, simp_all)+
+apply (rule disjI1)
+apply (simp add: prefixeq_def)
+apply (erule exE | erule conjE)+
+apply (rule_tac x="zs@zsa" in exI, simp)
+apply (rule_tac b=bb in comp_intro)
+apply (split cond_splits, simp_all)+
+apply (simp_all add: true_def)
+apply (erule disjE)
+apply (simp add: prefixeq_def)
+apply (erule exE | erule conjE)+
+apply (rule_tac x="zs@zsa" in exI, simp)
+apply (auto simp add: prefixeq_def)
+done
+
+
+lemma state_update_before_is_CSP4: 
+  assumes A : "relation_of Ac is CSP4 healthy"
+  shows "relation_of (state_update_before sc Ac) is CSP4 healthy"
+apply (auto simp: relation_of_state_update_before relation_of_Skip rp_defs design_defs fun_eq_iff CSP4_def)
+apply (rule_tac b=c in comp_intro)
+apply (rule_tac b=ba in comp_intro, simp_all)
+apply (split cond_splits, simp_all)
+apply (rule_tac b=bb in comp_intro, simp_all)
+apply (subst A[simplified design_defs rp_defs CSP4_def relation_of_Skip])
+apply (auto simp: rp_defs)
+done
+
+definition state_update_after :: "'\<sigma> relation \<Rightarrow> ('\<theta>::ev_eq,'\<sigma>) action \<Rightarrow> ('\<theta>,'\<sigma>) action"
+where "state_update_after sc Ac = action_of(relation_of Ac ;; R (true \<turnstile> (\<lambda>(A, A'). sc (more A, more A') & \<not>wait A' & tr A = tr A')))"
+
+lemma state_update_after_is_action: 
+"(relation_of Ac ;; R (true \<turnstile> (\<lambda>(A, A'). sc (more A, more A') & \<not>wait A' & tr A = tr A'))) \<in> {p. is_CSP_process p}"
+apply (simp)
+apply (rule seq_CSP)
+apply (auto simp: relation_of_CSP[simplified is_CSP_process_def])
+apply (rule rd_is_CSP, auto)
+done
+
+lemmas state_update_after_is_CSP = state_update_after_is_action[simplified]
+
+lemma relation_of_state_update_after:
+"relation_of (state_update_after sc Ac) = (relation_of Ac ;; R (true \<turnstile> (\<lambda>(A, A'). sc (more A, more A') & \<not>wait A' & tr A = tr A')))"
+by (simp add: state_update_after_def action_of_inverse state_update_after_is_CSP)
+
+lemma mono_state_update_after: "mono (state_update_after sc)"
+by (auto simp: mono_def less_eq_action ref_def relation_of_state_update_after design_defs rp_defs fun_eq_iff 
+            split: cond_splits dest: relation_of_spec_f_f[simplified] 
+                                     relation_of_spec_t_f[simplified])
+
+
+lemma state_update_after_is_CSP3: 
+  assumes A : "relation_of Ac is CSP3 healthy"
+  shows "relation_of (state_update_after sc Ac) is CSP3 healthy"
+apply (auto simp: relation_of_state_update_after relation_of_Skip rp_defs design_defs fun_eq_iff CSP3_def)
+apply (rule_tac b=aa in comp_intro)
+apply (split cond_splits, auto)
+apply (rule_tac b=bb in comp_intro, simp_all)
+apply (subst A[simplified design_defs rp_defs CSP3_def relation_of_Skip])
+apply (auto simp: rp_defs)
+done
+
+
+lemma state_update_after_is_CSP4: "relation_of (state_update_after sc Ac) is CSP4 healthy"
+apply (auto simp: relation_of_state_update_after relation_of_Skip rp_defs design_defs fun_eq_iff CSP4_def)
+apply (rule_tac b=c in comp_intro)
+apply (rule_tac b=ba in comp_intro, simp_all)
+apply (split cond_splits, simp_all)+
+apply (rule_tac b=bb in comp_intro, simp_all)
+apply (split cond_splits, simp_all)+
+apply (case_tac "ok bb", simp_all)
+apply (case_tac "tr bb \<le> tr c", simp_all)
+apply (case_tac "ok ca", simp_all)
+apply (case_tac "tr ca \<le> tr c", simp_all)
+apply (simp add: prefixeq_def)
+apply (erule exE)+
+apply (erule_tac x="zs@zsa" in allE, simp)
+apply (rule_tac b=bb in comp_intro, simp_all)
+apply (split cond_splits, simp_all add: true_def)+
+apply (case_tac "ok ca", simp_all)
+apply (case_tac "tr ca \<le> tr c", simp_all)
+apply (simp add: prefixeq_def)
+apply (erule exE | erule conjE)+
+apply (rule_tac x="zsa@zs" in exI, simp)
+apply (rule_tac b=bb in comp_intro, simp_all)
+apply (split cond_splits, simp_all)+
+apply (case_tac "tr bb \<le> tr c", simp_all)
+apply (simp add: prefixeq_def)
+apply (erule exE | erule conjE)+
+apply (erule_tac x="zsa@zs" in allE, simp)
+apply (auto simp add: prefixeq_def)
+done
+
+
+
+subsection {* Sequential composition *}
+
+definition 
+Seq::"('\<theta>::ev_eq,'\<sigma>) action \<Rightarrow> ('\<theta>,'\<sigma>) action \<Rightarrow> ('\<theta>,'\<sigma>) action" (infixl "`;`" 24)
+where "P `;` Q \<equiv> action_of (relation_of P ;; relation_of Q)"
+
+lemma Seq_is_action: "(relation_of P ;; relation_of Q) \<in> {p. is_CSP_process p}"
+apply (simp)
+apply (rule seq_CSP[OF relation_of_CSP[THEN CSP_is_CSP1] relation_of_CSP[THEN CSP_is_R] relation_of_CSP])
+done
+
+lemmas Seq_is_CSP = Seq_is_action[simplified]
+
+lemma relation_of_Seq: "relation_of (P `;` Q) = (relation_of P ;; relation_of Q)"
+by (simp add: Seq_def action_of_inverse Seq_is_CSP)
+
+lemma mono_Seq: "mono (op `;` P)"
+  by (auto simp: mono_def less_eq_action ref_def relation_of_Seq)
+
+
+lemma CSP3_imp_left_Skip:
+  assumes A: "relation_of P is CSP3 healthy"
+  shows "(Skip `;` P) = P"
+apply (subst relation_of_inject[symmetric])
+apply (simp add: relation_of_Seq A[simplified design_defs CSP3_def, symmetric])
+done
+
+lemma CSP4_imp_right_Skip:
+  assumes A: "relation_of P is CSP4 healthy"
+  shows "(P `;` Skip) = P"
+apply (subst relation_of_inject[symmetric])
+apply (simp add: relation_of_Seq A[simplified design_defs CSP4_def, symmetric])
+done
+
+lemma Seq_assoc: "(A `;` (B `;` C)) = ((A `;` B) `;` C)"
+by (auto simp: relation_of_inject[symmetric] fun_eq_iff relation_of_Seq rp_defs design_defs)
+
+lemma Skip_absorb: "(Skip `;` Skip) = Skip"
+by (auto simp: Skip_comp_absorb relation_of_inject[symmetric] relation_of_Seq)
+
+
+subsection {* Internal choice *}
 
 definition 
 Ndet::"('\<theta>::ev_eq,'\<sigma>) action \<Rightarrow> ('\<theta>,'\<sigma>) action \<Rightarrow> ('\<theta>,'\<sigma>) action" (infixl "\<sqinter>" 18) 
 where "P \<sqinter> Q \<equiv> action_of ((relation_of P) \<or> (relation_of Q))"
 
-lemma Ndet_is_action: "((relation_of P) \<or> (relation_of Q)) : action"
-apply (simp add: action_def)
+lemma Ndet_is_action: "((relation_of P) \<or> (relation_of Q)) \<in> {p. is_CSP_process p}"
+apply (simp)
 apply (rule disj_CSP)
 apply (simp_all add: relation_of_CSP)
 done
 
-lemmas Ndet_is_CSP = Ndet_is_action[simplified action_def]
+lemmas Ndet_is_CSP = Ndet_is_action[simplified]
 
 lemma relation_of_Ndet: "relation_of (P \<sqinter> Q) = ((relation_of P) \<or> (relation_of Q))"
-by (simp add: Ndet_def action_of_inverse Ndet_is_action)
+by (simp add: Ndet_def action_of_inverse Ndet_is_CSP)
 
 lemma mono_Ndet: "mono (op \<sqinter> P)"
 by (auto simp: mono_def less_eq_action ref_def relation_of_Ndet)
 
-subsubsection {* External choice *}
+subsection {* External choice *}
 
 definition
 Det::"('\<theta>::ev_eq,'\<sigma>) action \<Rightarrow> ('\<theta>,'\<sigma>) action \<Rightarrow> ('\<theta>,'\<sigma>) action" (infixl "[+]" 18)
-where "P [+] Q \<equiv> action_of(R((\<not>((relation_of P)\<^sup>f\<^sub>f) \<and> \<not>((relation_of Q)\<^sup>f\<^sub>f)) \<turnstile>
-                                             (((relation_of P)\<^sup>t\<^sub>f \<and> ((relation_of Q)\<^sup>t\<^sub>f))
+where "P [+] Q \<equiv> action_of(R((\<not>((relation_of P)\<^isup>f\<^isub>f) \<and> \<not>((relation_of Q)\<^isup>f\<^isub>f)) \<turnstile>
+                                             (((relation_of P)\<^isup>t\<^isub>f \<and> ((relation_of Q)\<^isup>t\<^isub>f))
                                                 \<triangleleft> \<lambda>(A, A'). tr A = tr A' \<and> wait A' \<triangleright>
-                                              ((relation_of P)\<^sup>t\<^sub>f \<or> ((relation_of Q)\<^sup>t\<^sub>f)))))"
+                                              ((relation_of P)\<^isup>t\<^isub>f \<or> ((relation_of Q)\<^isup>t\<^isub>f)))))"
 
 notation(xsymbol)
   Det (infixl "\<box>" 18)
 
 lemma Det_is_action: 
-"(R((\<not>((relation_of P)\<^sup>f\<^sub>f) \<and> \<not>((relation_of Q)\<^sup>f\<^sub>f)) \<turnstile>
-           (((relation_of P)\<^sup>t\<^sub>f \<and> ((relation_of Q)\<^sup>t\<^sub>f))
+"(R((\<not>((relation_of P)\<^isup>f\<^isub>f) \<and> \<not>((relation_of Q)\<^isup>f\<^isub>f)) \<turnstile>
+           (((relation_of P)\<^isup>t\<^isub>f \<and> ((relation_of Q)\<^isup>t\<^isub>f))
               \<triangleleft> \<lambda>(A, A'). tr A = tr A' \<and> wait A' \<triangleright>
-            ((relation_of P)\<^sup>t\<^sub>f \<or> ((relation_of Q)\<^sup>t\<^sub>f))))) : action"
-apply (simp add: action_def spec_def)
+            ((relation_of P)\<^isup>t\<^isub>f \<or> ((relation_of Q)\<^isup>t\<^isub>f))))) \<in> {p. is_CSP_process p}"
+apply (simp add: spec_def)
 apply (rule rd_is_CSP)
 apply (auto)
 done
 
-lemmas Det_is_CSP = Det_is_action[simplified action_def]
+lemmas Det_is_CSP = Det_is_action[simplified]
 
 lemma relation_of_Det:
-"relation_of (P \<box> Q) = (R((\<not>((relation_of P)\<^sup>f\<^sub>f) \<and> \<not>((relation_of Q)\<^sup>f\<^sub>f)) \<turnstile>
-                                          (((relation_of P)\<^sup>t\<^sub>f \<and> ((relation_of Q)\<^sup>t\<^sub>f))
+"relation_of (P \<box> Q) = (R((\<not>((relation_of P)\<^isup>f\<^isub>f) \<and> \<not>((relation_of Q)\<^isup>f\<^isub>f)) \<turnstile>
+                                          (((relation_of P)\<^isup>t\<^isub>f \<and> ((relation_of Q)\<^isup>t\<^isub>f))
                                              \<triangleleft> \<lambda>(A, A'). tr A = tr A' \<and> wait A' \<triangleright>
-                                           ((relation_of P)\<^sup>t\<^sub>f \<or> ((relation_of Q)\<^sup>t\<^sub>f)))))"
+                                           ((relation_of P)\<^isup>t\<^isub>f \<or> ((relation_of Q)\<^isup>t\<^isub>f)))))"
 apply (unfold Det_def)
 apply (rule action_of_inverse)
 apply (rule Det_is_action)
@@ -124,10 +410,43 @@ by (auto simp: mono_def less_eq_action ref_def relation_of_Det design_defs rp_de
             split: cond_splits dest: relation_of_spec_f_f[simplified] 
                                      relation_of_spec_t_f[simplified])
 
-subsubsection {* Schema expression *}
 
-definition Pre ::"'\<sigma> relation \<Rightarrow> '\<sigma> predicate"
-where "Pre sc \<equiv> \<lambda>A. \<exists> A'. sc (A, A')"
+subsection {* Reactive design assignment *}
+
+
+definition 
+"rd_assign s = action_of (R (true \<turnstile> \<lambda>(A, A'). ref A' = ref A \<and> tr A' = tr A \<and> \<not>wait A' \<and> more A' = s))"
+
+
+lemma rd_assign_is_action: 
+"(R (true \<turnstile> \<lambda>(A, A'). ref A' = ref A \<and> tr A' = tr A \<and> \<not>wait A' \<and> more A' = s)) \<in> {p. is_CSP_process p}"
+apply (auto simp:)
+apply (rule rd_is_CSP)
+by auto
+
+lemmas rd_assign_is_CSP = rd_assign_is_action[simplified]
+
+lemma relation_of_rd_assign: 
+"relation_of (rd_assign s) = 
+                  (R (true \<turnstile> \<lambda>(A, A'). ref A' = ref A \<and> tr A' = tr A \<and> \<not>wait A' \<and> more A' = s))"
+by (simp add: rd_assign_def  action_of_inverse rd_assign_is_CSP)
+
+
+
+
+
+subsection {* Local state external choice *}
+
+definition
+Loc::"'\<sigma> \<Rightarrow> ('\<theta>::ev_eq,'\<sigma>) action \<Rightarrow> '\<sigma> \<Rightarrow> ('\<theta>,'\<sigma>) action \<Rightarrow> ('\<theta>,'\<sigma>) action" 
+                                        ("'(()loc _ \<bullet> _ ') \<boxplus> '(()loc _ \<bullet> _ ')")
+where "(loc s1 \<bullet> P) \<boxplus> (loc s2 \<bullet> Q) \<equiv> 
+                   ((rd_assign s1)`;`P) \<box> ((rd_assign s2)`;` Q)"
+
+
+
+subsection {* Schema expression *}
+
 
 definition Schema :: "'\<sigma> relation \<Rightarrow> ('\<theta>::ev_eq,'\<sigma>) action" where
 "Schema sc \<equiv> action_of(R ((\<lambda>(A, A'). (Pre sc) (more A)) \<turnstile> 
@@ -135,39 +454,36 @@ definition Schema :: "'\<sigma> relation \<Rightarrow> ('\<theta>::ev_eq,'\<sigm
 
 lemma Schema_is_action: 
 "(R ((\<lambda>(A, A'). (Pre sc) (more A)) \<turnstile> 
-                 (\<lambda>(A, A'). sc (more A, more A') \<and> \<not>wait A' \<and> tr A = tr A'))) : action"
-apply (simp add: action_def)
+                 (\<lambda>(A, A'). sc (more A, more A') & \<not>wait A' & tr A = tr A'))) \<in> {p. is_CSP_process p}"
+apply (simp)
 apply (rule rd_is_CSP)
 apply (auto)
 done
 
-lemmas Schema_is_CSP = Schema_is_action[simplified action_def]
+lemmas Schema_is_CSP = Schema_is_action[simplified]
 
 lemma relation_of_Schema:
 "relation_of (Schema sc) = (R ((\<lambda>(A, A'). (Pre sc) (more A)) \<turnstile> 
                           (\<lambda>(A, A'). sc (more A, more A') \<and> \<not>wait A' \<and> tr A = tr A')))"
-by (simp add: Schema_def action_of_inverse Schema_is_action)
+by (simp add: Schema_def action_of_inverse Schema_is_CSP)
 
-subsubsection {* Sequential composition *}
-
-definition 
-Seq::"('\<theta>::ev_eq,'\<sigma>) action \<Rightarrow> ('\<theta>,'\<sigma>) action \<Rightarrow> ('\<theta>,'\<sigma>) action" (infixl "`;`" 24)
-where "P `;` Q \<equiv> action_of (relation_of P ;; relation_of Q)"
-
-lemma Seq_is_action: "(relation_of P ;; relation_of Q) : action"
-apply (simp add: action_def)
-apply (rule seq_CSP[OF relation_of_CSP[THEN CSP_is_CSP1] relation_of_CSP[THEN CSP_is_R] relation_of_CSP])
+lemma Schema_is_state_update_before: "Schema u = state_update_before u Skip"
+apply (subst relation_of_inject[symmetric])
+apply (auto simp: relation_of_Schema relation_of_state_update_before relation_of_Skip rp_defs fun_eq_iff
+                  design_defs)
+apply (split cond_splits, simp_all)
+apply (rule comp_intro)
+apply (split cond_splits, simp_all)+
+apply (rule comp_intro)
+apply (split cond_splits, simp_all)+
+prefer 3
+apply (split cond_splits, simp_all)+
+apply (auto simp: prefixeq_def)
 done
 
-lemmas Seq_is_CSP = Seq_is_action[simplified action_def]
 
-lemma relation_of_Seq: "relation_of (P `;` Q) = (relation_of P ;; relation_of Q)"
-by (simp add: Seq_def action_of_inverse Seq_is_action)
 
-lemma mono_Seq: "mono (op `;` P)"
-  by (auto simp: mono_def less_eq_action ref_def relation_of_Seq)
-
-subsubsection {* Parallel composition *}
+subsection {* Parallel composition *}
 
 type_synonym '\<sigma> local_state = "('\<sigma> \<times> ('\<sigma>  \<Rightarrow> '\<sigma> \<Rightarrow> '\<sigma>))"
 
@@ -184,9 +500,9 @@ fun ParMergel :: "'\<theta>::ev_eq list \<Rightarrow> '\<theta> list \<Rightarro
                                           else (b ## (ParMergel [] tr2 cs)))" 
   | "ParMergel (a#tr1) [] cs = (if (filter_chan_set a cs) then [[]]
                                           else (a ## (ParMergel tr1 [] cs)))"
-  | "ParMergel (a#tr1) (b#tr2) cs = 
+  | "ParMergel (a#tr1) (b#tr2) cs =
            (if (filter_chan_set a cs)
-                   then (if (ev_eq a b) 
+                   then (if (ev_eq a b)
                               then (a ## (ParMergel tr1 tr2 cs)) 
                                else (if (filter_chan_set b cs) 
                                         then [[]] 
@@ -199,11 +515,19 @@ fun ParMergel :: "'\<theta>::ev_eq list \<Rightarrow> '\<theta> list \<Rightarro
 definition ParMerge::"'\<theta>::ev_eq list \<Rightarrow> '\<theta> list \<Rightarrow> '\<theta> set \<Rightarrow> '\<theta> list set" where
 "ParMerge tr1 tr2 cs = set (ParMergel tr1 tr2 cs)"
 
+lemma set_Cons1: "tr1 \<in> set l \<Longrightarrow> a # tr1 \<in> op # a ` set l"
+by (auto)
+
+lemma tr_in_set_eq: "(tr1 \<in> op # b ` set l) = (tr1 \<noteq> [] \<and> hd tr1 = b \<and> tl tr1 \<in> set l)"
+by (induct l) auto
+
+
+
 definition M_par::"(('\<theta>::ev_eq), '\<sigma>) alpha_rp_scheme \<Rightarrow> ('\<sigma>  \<Rightarrow> '\<sigma> \<Rightarrow> '\<sigma>)
                             \<Rightarrow> ('\<theta>, '\<sigma>) alpha_rp_scheme \<Rightarrow> ('\<sigma> \<Rightarrow> '\<sigma> \<Rightarrow> '\<sigma>)
                                 \<Rightarrow> ('\<theta> set) \<Rightarrow> ('\<theta>, '\<sigma>) relation_rp" where
 "M_par s1 x1 s2 x2 cs = 
-((\<lambda>(S, S'). ((diff_tr S' S) \<in> ParMerge (diff_tr s1 S) (diff_tr s2 S) cs \<and>
+((\<lambda>(S, S'). ((diff_tr S' S) \<in> ParMerge (diff_tr s1 S) (diff_tr s2 S) cs &
      ev_eq (tr_filter (tr s1) cs) (tr_filter (tr s2) cs))) \<and>
    ((\<lambda>(S, S'). (wait s1 \<or> wait s2) \<and> 
                              ref S' \<subseteq> ((((ref s1)\<union>(ref s2))\<inter>cs)\<union>(((ref s1)\<inter>(ref s2))-cs)))
@@ -214,41 +538,41 @@ definition  Par::"('\<theta>::ev_eq,'\<sigma>) action \<Rightarrow>
                     ('\<sigma>  \<Rightarrow> '\<sigma> \<Rightarrow> '\<sigma>) \<Rightarrow> '\<theta> set \<Rightarrow> ('\<sigma>  \<Rightarrow> '\<sigma> \<Rightarrow> '\<sigma>) \<Rightarrow> 
                     ('\<theta>,'\<sigma>) action \<Rightarrow> ('\<theta>,'\<sigma>) action" ("_ \<lbrakk> _ | _ | _ \<rbrakk> _") where
 "A1 \<lbrakk> ns1 | cs | ns2 \<rbrakk> A2 \<equiv> (action_of (R ((\<lambda> (S, S'). 
- \<not> (\<exists> tr1 tr2. ((relation_of A1)\<^sup>f\<^sub>f ;; (\<lambda> (S, S'). tr1 = (tr S))) (S, S') 
+ \<not> (\<exists> tr1 tr2. ((relation_of A1)\<^isup>f\<^isub>f ;; (\<lambda> (S, S'). tr1 = (tr S))) (S, S') 
  \<and> (spec False (wait S) (relation_of A2) ;; (\<lambda> (S, _). tr2 = (tr S))) (S, S')
  \<and> ((tr_filter tr1 cs) = (tr_filter tr2 cs))) \<and>
  \<not> (\<exists> tr1 tr2. (spec False (wait S) (relation_of A1);;(\<lambda>(S, _). tr1 = tr S)) (S, S')
- \<and> ((relation_of A2)\<^sup>f\<^sub>f ;; (\<lambda>(S, S'). tr2 = (tr S))) (S, S') 
+ \<and> ((relation_of A2)\<^isup>f\<^isub>f ;; (\<lambda>(S, S'). tr2 = (tr S))) (S, S') 
  \<and> ((tr_filter tr1 cs) = (tr_filter tr2 cs)))) \<turnstile> 
-   (\<lambda> (S, S'). (\<exists> s1 s2. ((\<lambda> (A, A'). (relation_of A1)\<^sup>t\<^sub>f (A, s1)
- \<and> ((relation_of A2)\<^sup>t\<^sub>f (A, s2)));; M_par s1 ns1 s2 ns2 cs) (S, S'))))))"
+   (\<lambda> (S, S'). (\<exists> s1 s2. ((\<lambda> (A, A'). (relation_of A1)\<^isup>t\<^isub>f (A, s1)
+ \<and> ((relation_of A2)\<^isup>t\<^isub>f (A, s2)));; M_par s1 ns1 s2 ns2 cs) (S, S'))))))"
 
 lemma Par_is_action: "(R ((\<lambda> (S, S'). 
- \<not> (\<exists> tr1 tr2. ((relation_of A1)\<^sup>f\<^sub>f ;; (\<lambda> (S, S'). tr1 = (tr S))) (S, S') 
+ \<not> (\<exists> tr1 tr2. ((relation_of A1)\<^isup>f\<^isub>f ;; (\<lambda> (S, S'). tr1 = (tr S))) (S, S') 
  \<and> (spec False (wait S) (relation_of A2) ;; (\<lambda> (S, S'). tr2 = (tr S))) (S, S')
  \<and> ((tr_filter tr1 cs) = (tr_filter tr2 cs))) \<and>
  \<not> (\<exists> tr1 tr2. (spec False (wait S) (relation_of A1);;(\<lambda>(S, _). tr1 = tr S)) (S, S')
- \<and> ((relation_of A2)\<^sup>f\<^sub>f ;; (\<lambda> (S, S'). tr2 = (tr S))) (S, S') 
+ \<and> ((relation_of A2)\<^isup>f\<^isub>f ;; (\<lambda> (S, S'). tr2 = (tr S))) (S, S') 
  \<and> ((tr_filter tr1 cs) = (tr_filter tr2 cs)))) \<turnstile> 
-   (\<lambda> (S, S'). (\<exists> s1 s2. ((\<lambda> (A, A'). (relation_of A1)\<^sup>t\<^sub>f (A, s1)
- \<and> ((relation_of A2)\<^sup>t\<^sub>f (A, s2)));; M_par s1 ns1 s2 ns2 cs) (S, S'))))) : action"
-apply (simp add: action_def)
+   (\<lambda> (S, S'). (\<exists> s1 s2. ((\<lambda> (A, A'). (relation_of A1)\<^isup>t\<^isub>f (A, s1)
+ \<and> ((relation_of A2)\<^isup>t\<^isub>f (A, s2)));; M_par s1 ns1 s2 ns2 cs) (S, S'))))) \<in> {p. is_CSP_process p}"
+apply (simp)
 apply (rule rd_is_CSP)
 apply (blast)
 done
 
-lemmas Par_is_CSP = Par_is_action[simplified action_def]
+lemmas Par_is_CSP = Par_is_action[simplified]
 
 lemma relation_of_Par:
 "relation_of (A1 \<lbrakk> ns1 | cs | ns2 \<rbrakk> A2) = (R ((\<lambda> (S, S'). 
- \<not> (\<exists> tr1 tr2. ((relation_of A1)\<^sup>f\<^sub>f ;; (\<lambda> (S, S'). tr1 = (tr S))) (S, S') 
+ \<not> (\<exists> tr1 tr2. ((relation_of A1)\<^isup>f\<^isub>f ;; (\<lambda> (S, S'). tr1 = (tr S))) (S, S') 
  \<and> (spec False (wait S) (relation_of A2) ;; (\<lambda> (S, S'). tr2 = (tr S))) (S, S') 
  \<and> ((tr_filter tr1 cs) = (tr_filter tr2 cs))) \<and>
  \<not> (\<exists> tr1 tr2. (spec False (wait S) (relation_of A1);;(\<lambda>(S, _). tr1 = tr S)) (S, S') 
- \<and> ((relation_of A2)\<^sup>f\<^sub>f ;; (\<lambda> (S, S'). tr2 = (tr S))) (S, S') 
+ \<and> ((relation_of A2)\<^isup>f\<^isub>f ;; (\<lambda> (S, S'). tr2 = (tr S))) (S, S') 
  \<and> ((tr_filter tr1 cs) = (tr_filter tr2 cs)))) \<turnstile> 
-   (\<lambda> (S, S'). (\<exists> s1 s2. ((\<lambda> (A, A'). (relation_of A1)\<^sup>t\<^sub>f (A, s1)
- \<and> ((relation_of A2)\<^sup>t\<^sub>f (A, s2)));; M_par s1 ns1 s2 ns2 cs) (S, S')))))"
+   (\<lambda> (S, S'). (\<exists> s1 s2. ((\<lambda> (A, A'). (relation_of A1)\<^isup>t\<^isub>f (A, s1)
+ \<and> ((relation_of A2)\<^isup>t\<^isub>f (A, s2)));; M_par s1 ns1 s2 ns2 cs) (S, S')))))"
 apply (unfold Par_def)
 apply (rule action_of_inverse)
 apply (rule Par_is_action)
@@ -263,43 +587,18 @@ lemma mono_Par: "mono (\<lambda>Q. P \<lbrakk> ns1 | cs | ns2 \<rbrakk> Q)"
   apply (auto dest: relation_of_spec_f_f relation_of_spec_t_f)
 done
 
-subsubsection {* Assignment *}
-text {* Circus variables are represented by a stack (list) of values. 
-they are characterized by two functions, $select$ and $update$.
-The Circus variable type is defined as a tuple ($select$ * $update$) with a 
-list of values instead of a single value. *}
 
-type_synonym ('a, '\<sigma>) var_list = "('\<sigma> \<Rightarrow> 'a list) * (('a list \<Rightarrow> 'a list) \<Rightarrow> '\<sigma> \<Rightarrow> '\<sigma>)"
+subsection {* Local parallel block *}
 
-text {* The $select$ function returns the top value of the stack. *}
+definition
+ParLoc::"'\<sigma> \<Rightarrow> ('\<sigma> \<Rightarrow> '\<sigma> \<Rightarrow> '\<sigma>) \<Rightarrow> ('\<theta>::ev_eq, '\<sigma>) action \<Rightarrow> '\<theta> set \<Rightarrow> '\<sigma> \<Rightarrow> ('\<sigma> \<Rightarrow> '\<sigma> \<Rightarrow> '\<sigma>) \<Rightarrow> ('\<theta>,'\<sigma>) action \<Rightarrow> ('\<theta>,'\<sigma>) action"
+                                        ("'(()par _ | _ \<bullet> _ ') \<lbrakk> _ \<rbrakk> '(()par _ | _ \<bullet> _ ')")
+where 
+"(par s1 | ns1 \<bullet> P) \<lbrakk> cs \<rbrakk> (par s2 | ns2 \<bullet> Q) \<equiv> ((rd_assign s1)`;`P) \<lbrakk> ns1 | cs | ns2 \<rbrakk> ((rd_assign s2)`;` Q)"
 
-definition select :: "('a, 'r) var_list \<Rightarrow> 'r \<Rightarrow> 'a"
-where "select f \<equiv> \<lambda> A. hd ((fst f) A)"
 
-text {* The $increase$ function pushes a new value to the top of the stack. *}
 
-definition increase :: "('a, 'r) var_list \<Rightarrow> 'a \<Rightarrow> 'r \<Rightarrow> 'r"
-where "increase f val \<equiv> (snd f) (\<lambda> l. val#l)"
-
-text {* The $decrease$ function pops the top value of the stack. *}
-
-definition decrease :: "('a, 'r) var_list \<Rightarrow> 'r \<Rightarrow> 'r"
-where "decrease f \<equiv> (snd f) (\<lambda> l. (tl l))"
-
-text {* The $update$ function updates the top value of the stack. *}
-
-definition update :: "('a, 'r) var_list \<Rightarrow> ('a \<Rightarrow> 'a) \<Rightarrow> 'r \<Rightarrow> 'r"
-where "update f upd \<equiv> (snd f) (\<lambda> l. (upd (hd l))#(tl l))"
-
-text {* The $update0$ function initializes the top of the stack with an arbitrary value. *}
-
-definition update0 :: "('a, 'r) var_list \<Rightarrow> 'r \<Rightarrow> 'r"
-where "update0 f \<equiv> (snd f) (\<lambda> l. ((SOME upd. True) (hd l))#(tl l))"
-
-text {* The $VAR-LIST$ function allows to retrieve a Circus variable from its name.*}
-
-syntax "_VAR_LIST" :: "id \<Rightarrow> ('a, 'r) var_list"  ("VAR'_LIST _")
-translations "VAR_LIST x" => "(x, _update_name x)"
+subsection {* Assignment *}
 
 definition ASSIGN::"('v, '\<sigma>) var_list \<Rightarrow> ('\<sigma> \<Rightarrow> 'v) \<Rightarrow> ('\<theta>::ev_eq, '\<sigma>) action" where
 "ASSIGN x e \<equiv> action_of (R (true \<turnstile> (\<lambda> (S, S'). tr S' = tr S \<and> \<not>wait S' \<and> 
@@ -310,74 +609,180 @@ translations "y `:=` vv" => "CONST ASSIGN (VAR y) vv"
 
 lemma Assign_is_action: 
 "(R (true \<turnstile> (\<lambda> (S, S'). tr S' = tr S \<and> \<not>wait S' \<and> 
-                (more S' = (update x (\<lambda>_. (e (more S)))) (more S))))) : action"
-apply (simp add: action_def)
+                (more S' = (update x (\<lambda>_. (e (more S)))) (more S))))) \<in> {p. is_CSP_process p}"
+apply (simp)
 apply (rule rd_is_CSP)
 apply (blast)
 done
 
-lemmas Assign_is_CSP = Assign_is_action[simplified action_def]
+lemmas Assign_is_CSP = Assign_is_action[simplified]
 
 lemma relation_of_Assign:
 "relation_of (ASSIGN x e) = (R (true \<turnstile> (\<lambda> (S, S'). tr S' = tr S \<and> \<not>wait S' \<and> 
                                    (more S' = (update x (\<lambda>_. (e (more S)))) (more S)))))"
-by (simp add: ASSIGN_def action_of_inverse Assign_is_action)
+by (simp add: ASSIGN_def action_of_inverse Assign_is_CSP)
 
-subsubsection {* Variable scope *}
+lemma Assign_is_state_update_before: "ASSIGN x e = state_update_before (\<lambda> (s, s') . s' = (update x (\<lambda>_. (e s))) s) Skip"
+apply (subst relation_of_inject[symmetric])
+apply (auto simp: relation_of_Assign relation_of_state_update_before relation_of_Skip rp_defs fun_eq_iff
+                  Pre_def update_def design_defs)
+apply (split cond_splits, simp_all)+
+apply (rule_tac b=b in comp_intro)
+apply (split cond_splits, simp_all)+
+apply (rule_tac b=b in comp_intro)
+apply (split cond_splits, simp_all)+
+defer
+apply (split cond_splits, simp_all)+
+prefer 3
+apply (split cond_splits, simp_all)+
+apply (auto simp add: prefixeq_def)
+done
+
+
+subsection {* Variable scope *}
 
 definition Var::"('v, '\<sigma>) var_list \<Rightarrow>('\<theta>, '\<sigma>) action \<Rightarrow> ('\<theta>::ev_eq,'\<sigma>) action" where
 "Var v A \<equiv> action_of(
-     (R(true \<turnstile> (\<lambda> (A, A'). (\<exists> x. A' = A\<lparr>more := (increase v x (more A))\<rparr>))));; 
-     relation_of A;; 
-     (R(true \<turnstile> (\<lambda> (A, A'). A' = A\<lparr>more := (decrease v (more A))\<rparr>))))"
+     (R(true \<turnstile> (\<lambda> (A, A'). \<exists> a. tr A' = tr A \<and> \<not>wait A' \<and> more A' = (increase v a (more A)))));; 
+     (relation_of A;;
+     (R(true \<turnstile> (\<lambda> (A, A').  tr A' = tr A \<and> \<not>wait A' \<and> more A' = (decrease v (more A)))))))"
 
 syntax "_var"::"idt \<Rightarrow> ('\<theta>, '\<sigma>) action \<Rightarrow> ('\<theta>, '\<sigma>) action" ("var _ \<bullet> _" [1000] 999)
 translations "var y \<bullet> Act" => "CONST Var (VAR_LIST y) Act"
 
 lemma Var_is_action:
-"((R(true \<turnstile> (\<lambda> (A, A'). (\<exists> x. A' = A\<lparr>more := (increase v x (more A))\<rparr>))));;
-  relation_of A;; 
-  (R(true \<turnstile> (\<lambda> (A, A'). A' = A\<lparr>more := (decrease v (more A))\<rparr>)))) : action"
-  apply (simp add: action_def)
+"((R(true \<turnstile> (\<lambda> (A, A'). \<exists> a. tr A' = tr A \<and> \<not>wait A' \<and> more A' = (increase v a (more A)))));; 
+     (relation_of A;;
+     (R(true \<turnstile> (\<lambda> (A, A').  tr A' = tr A \<and> \<not>wait A' \<and> more A' = (decrease v (more A))))))) \<in> {p. is_CSP_process p}"
+  apply (simp)
   apply (rule seq_CSP)
   prefer 3
   apply (rule seq_CSP)
   apply (auto simp: relation_of_CSP1 relation_of_R)
   apply (rule rd_is_CSP)
-  apply (auto simp: csp_defs rp_defs design_defs fun_eq_iff prefix_def increase_def decrease_def
+  apply (auto simp: csp_defs rp_defs design_defs fun_eq_iff prefixeq_def increase_def decrease_def
                split: cond_splits)
 done
 
-lemmas Var_is_CSP = Var_is_action[simplified action_def]
+lemmas Var_is_CSP = Var_is_action[simplified]
 
 lemma relation_of_Var:
 "relation_of (Var v A) = 
-    ((R(true \<turnstile> (\<lambda> (A, A'). (\<exists> x. A' = A\<lparr>more := (increase v x (more A))\<rparr>))));; 
-     relation_of A;; 
-     (R(true \<turnstile> (\<lambda> (A, A'). A' = A\<lparr>more := (decrease v (more A))\<rparr>))))"
-by (simp add: Var_def action_of_inverse Var_is_action)
+    ((R(true \<turnstile> (\<lambda> (A, A'). \<exists> a. tr A' = tr A \<and> \<not>wait A' \<and> more A' = (increase v a (more A)))));; 
+     (relation_of A;;
+     (R(true \<turnstile> (\<lambda> (A, A').  tr A' = tr A \<and> \<not>wait A' \<and> more A' = (decrease v (more A)))))))"
+apply (simp only: Var_def)
+apply (rule action_of_inverse)
+apply (rule Var_is_action)
+done
+
 
 lemma mono_Var : "mono (Var x)"
   by (auto simp: mono_def less_eq_action ref_def relation_of_Var)
 
-subsubsection {* Guarded action *}
+
+
+definition Let::"('v, '\<sigma>) var_list \<Rightarrow>('\<theta>, '\<sigma>) action \<Rightarrow> ('\<theta>::ev_eq,'\<sigma>) action" where
+"Let v A \<equiv> action_of((relation_of A;;
+     (R(true \<turnstile> (\<lambda> (A, A').  tr A' = tr A \<and> \<not>wait A' \<and> more A' = (decrease v (more A)))))))"
+
+syntax "_let"::"idt \<Rightarrow> ('\<theta>, '\<sigma>) action \<Rightarrow> ('\<theta>, '\<sigma>) action" ("let _ \<bullet> _" [1000] 999)
+translations "let y \<bullet> Act" => "CONST Let (VAR_LIST y) Act"
+
+lemma Let_is_action:
+"(relation_of A;;
+     (R(true \<turnstile> (\<lambda> (A, A').  tr A' = tr A \<and> \<not>wait A' \<and> more A' = (decrease v (more A)))))) \<in> {p. is_CSP_process p}"
+  apply (simp)
+  apply (rule seq_CSP)
+  apply (auto simp: relation_of_CSP1 relation_of_R)
+  apply (rule rd_is_CSP)
+  apply (auto)
+done
+
+lemmas Let_is_CSP = Let_is_action[simplified]
+
+lemma relation_of_Let:
+"relation_of (Let v A) = 
+    (relation_of A;;
+     (R(true \<turnstile> (\<lambda> (A, A').  tr A' = tr A \<and> \<not>wait A' \<and> more A' = (decrease v (more A))))))"
+by (simp add: Let_def action_of_inverse Let_is_CSP)
+
+lemma mono_Let : "mono (Let x)"
+  by (auto simp: mono_def less_eq_action ref_def relation_of_Let)
+
+
+lemma Var_is_state_update_before: "Var v A = state_update_before (\<lambda> (s, s'). \<exists> a. s' = increase v a s) (Let v A)"
+apply (subst relation_of_inject[symmetric])
+apply (auto simp: relation_of_Var relation_of_Let relation_of_state_update_before relation_of_Skip fun_eq_iff)
+apply (auto simp: rp_defs fun_eq_iff Pre_def design_defs)
+apply (split cond_splits, simp_all)+
+apply (rule_tac b=ab in comp_intro)
+apply (split cond_splits, simp_all)+
+apply (rule_tac b=bb in comp_intro, simp_all)
+apply (split cond_splits, simp_all)+
+apply (rule_tac b=ab in comp_intro)
+apply (split cond_splits, simp_all)+
+apply (rule_tac b=bb in comp_intro, simp_all)
+apply (split cond_splits, simp_all)+
+apply (rule_tac b=ab in comp_intro)
+apply (split cond_splits, simp_all)+ defer
+apply (rule_tac b=bb in comp_intro, simp_all)
+apply (split cond_splits, simp_all)+
+apply (rule_tac b=ab in comp_intro)
+apply (split cond_splits, simp_all)+ defer
+apply (rule_tac b=bb in comp_intro, simp_all)
+apply (split cond_splits, simp_all)+
+apply (rule_tac b=ab in comp_intro)
+apply (split cond_splits, simp_all)+
+apply (rule_tac b=bb in comp_intro, simp_all)
+apply (split cond_splits, simp_all)+
+apply (rule_tac b=ab in comp_intro)
+apply (split cond_splits, simp_all)+
+apply (rule_tac b=bb in comp_intro, simp_all)
+apply (split cond_splits, simp_all)+
+apply (rule_tac b=ab in comp_intro)
+apply (split cond_splits, simp_all)+
+apply (case_tac "\<exists>A' a. A' = increase v a (alpha_rp.more aa)", simp_all add: true_def)
+apply (erule_tac x="increase v a (alpha_rp.more aa)" in allE)
+apply (erule_tac x="a" in allE, simp)
+apply (rule_tac b=bb in comp_intro, simp_all)
+apply (split cond_splits, simp_all)+
+apply (rule_tac b=ab in comp_intro)
+apply (split cond_splits, simp_all)+
+apply (case_tac "\<exists>A' a. A' = increase v a (alpha_rp.more aa)", simp_all add: true_def)
+apply (erule_tac x="increase v a (alpha_rp.more aa)" in allE)
+apply (erule_tac x="a" in allE, simp)
+apply (rule_tac b=bb in comp_intro, simp_all)
+apply (split cond_splits, simp_all)+
+done
+
+
+lemma Let_is_state_update_after: "Let v A = state_update_after (\<lambda> (s, s'). s' = decrease v s) A"
+apply (subst relation_of_inject[symmetric])
+apply (auto simp: relation_of_Var relation_of_Let relation_of_state_update_after relation_of_Skip fun_eq_iff)
+apply (auto simp: rp_defs fun_eq_iff Pre_def design_defs)
+apply (auto split: cond_splits)
+done
+
+
+subsection {* Guarded action *}
 
 definition Guard::"'\<sigma> predicate \<Rightarrow> ('\<theta>::ev_eq, '\<sigma>) action \<Rightarrow> ('\<theta>, '\<sigma>) action" ("_ `&` _")
-where "g `&` P \<equiv> action_of(R (((g o more o fst) \<longrightarrow> \<not> ((relation_of P)\<^sup>f\<^sub>f)) \<turnstile> 
-                             (((g o more o fst) \<and> ((relation_of P)\<^sup>t\<^sub>f)) \<or> 
+where "g `&` P \<equiv> action_of(R (((g o more o fst) \<longrightarrow> \<not> ((relation_of P)\<^isup>f\<^isub>f)) \<turnstile> 
+                             (((g o more o fst) \<and> ((relation_of P)\<^isup>t\<^isub>f)) \<or> 
                          ((\<not>(g o more o fst)) \<and> (\<lambda> (A, A'). tr A' = tr A \<and> wait A')))))"
 
 lemma Guard_is_action: 
-"(R ( ((g o more o fst) \<longrightarrow> \<not> ((relation_of P)\<^sup>f\<^sub>f)) \<turnstile> 
-                (((g o more o fst) \<and> ((relation_of P)\<^sup>t\<^sub>f)) \<or> 
-                 ((\<not>(g o more o fst)) \<and> (\<lambda> (A, A'). tr A' = tr A \<and> wait A'))))) : action"
-  by (auto simp add: action_def spec_def intro: rd_is_CSP)
+"(R ( ((g o more o fst) \<longrightarrow> \<not> ((relation_of P)\<^isup>f\<^isub>f)) \<turnstile> 
+                (((g o more o fst) \<and> ((relation_of P)\<^isup>t\<^isub>f)) \<or> 
+                 ((\<not>(g o more o fst)) \<and> (\<lambda> (A, A'). tr A' = tr A \<and> wait A'))))) \<in> {p. is_CSP_process p}"
+  by (auto simp add: spec_def intro: rd_is_CSP)
 
-lemmas Guard_is_CSP = Guard_is_action[simplified action_def]
+lemmas Guard_is_CSP = Guard_is_action[simplified]
 
 lemma relation_of_Guard:
-"relation_of (g `&` P) = (R (((g o more o fst) \<longrightarrow>  \<not> ((relation_of P)\<^sup>f\<^sub>f)) \<turnstile> 
-                             (((g o more o fst) \<and> ((relation_of P)\<^sup>t\<^sub>f)) \<or>
+"relation_of (g `&` P) = (R (((g o more o fst) \<longrightarrow>  \<not> ((relation_of P)\<^isup>f\<^isub>f)) \<turnstile> 
+                             (((g o more o fst) \<and> ((relation_of P)\<^isup>t\<^isub>f)) \<or>
                           ((\<not>(g o more o fst)) \<and> (\<lambda> (A, A'). tr A' = tr A \<and> wait A')))))"
   apply (unfold Guard_def)
   apply (subst action_of_inverse)
@@ -418,33 +823,80 @@ apply (subst CSP_is_rd[OF relation_of_CSP]) back back
 apply (auto simp: fun_eq_iff csp_defs design_defs rp_defs split: cond_splits)
 done
 
-subsubsection {* Prefixed action *}
+lemma Guard_is_state_update_before: "g `&` P = state_update_before (\<lambda> (s, s') . g s) P"
+apply (subst relation_of_inject[symmetric])
+apply (auto simp: relation_of_Guard relation_of_state_update_before relation_of_Skip rp_defs fun_eq_iff
+                  Pre_def update_def design_defs)
+apply (rule_tac b=a in comp_intro)
+apply (split cond_splits, simp_all)+
+apply (subst CSP_is_rd)
+apply (simp_all add: relation_of_CSP rp_defs design_defs fun_eq_iff)
+apply (split cond_splits, simp_all)+
+apply (auto)
+apply (subst (asm) CSP_is_rd)
+apply (simp_all add: relation_of_CSP rp_defs design_defs fun_eq_iff)
+apply (split cond_splits, simp_all)+
+apply (subst (asm) CSP_is_rd)
+apply (simp_all add: relation_of_CSP rp_defs design_defs fun_eq_iff)
+apply (split cond_splits, simp_all)+
+apply (subst CSP_is_rd)
+apply (simp_all add: relation_of_CSP rp_defs design_defs fun_eq_iff)
+apply (split cond_splits, simp_all)+
+apply (subst CSP_is_rd)
+apply (simp_all add: relation_of_CSP rp_defs design_defs fun_eq_iff)
+apply (split cond_splits, simp_all)+
+apply (auto) defer
+apply (split cond_splits, simp_all)+
+apply (subst (asm) CSP_is_rd)
+apply (simp_all add: relation_of_CSP rp_defs design_defs fun_eq_iff)
+apply (split cond_splits, simp_all)+ defer
+apply (rule disjI1) defer
+apply (case_tac "g (alpha_rp.more aa)", simp_all)
+apply (rule)+
+apply (simp add: impl_def) defer
+oops
+
+subsection {* Prefixed action *}
 
 definition do where
-"do e \<equiv> (\<lambda>(A, A'). tr A = tr A' \<and> e \<notin> (ref A')) \<triangleleft> wait o fst \<triangleright> 
-                                                              (\<lambda>(A, A'). tr A' = (tr A @[e]))"
+"do e \<equiv> (\<lambda>(A, A'). tr A = tr A' \<and> (e (more A)) \<notin> (ref A')) \<triangleleft> wait o snd \<triangleright> 
+         (\<lambda>(A, A'). tr A' = (tr A @[(e (more A))]))"
 
+definition do_I::"('\<sigma> \<Rightarrow>'\<theta>) \<Rightarrow> '\<theta> set \<Rightarrow> ('\<theta>, '\<sigma>) relation_rp"
+where "do_I c S \<equiv>  ((\<lambda>(A, A'). tr A = tr A' & S \<inter> (ref A') = {})
+                                \<triangleleft> wait o snd \<triangleright> 
+  (\<lambda>(A, A'). hd (tr A' - tr A) \<in> S & (c (more A) = (last (tr A')))))"
+
+(*
 definition do_I::"('v \<Rightarrow> '\<theta>) \<Rightarrow> ('v, '\<sigma>) var_list \<Rightarrow> 'v set \<Rightarrow> ('\<theta>, '\<sigma>) relation_rp"
 where "do_I c x P \<equiv>  ((\<lambda>(A, A'). tr A = tr A' \<and> (c`P) \<inter> (ref A') = {})
                                 \<triangleleft> wait o fst \<triangleright> 
   (\<lambda>(A, A'). hd (tr A' - tr A) \<in> (c`P) \<and> (c (select x (more A)) = (last (tr A')))))"
+*)
+
 
 definition
-Prefix::"('v \<Rightarrow> '\<theta>) \<Rightarrow> ('v, '\<sigma>) var_list \<Rightarrow> 'v set \<Rightarrow> ('\<theta>::ev_eq, '\<sigma>) action 
-                                                                           \<Rightarrow> ('\<theta>, '\<sigma>) action" where
-"Prefix c x S P \<equiv> action_of(R(true \<turnstile> (do_I c x S) \<and> 
-                                                    (\<lambda> (A, A'). more A' = more A)))`;` P"
+iPrefix::"('\<sigma> \<Rightarrow>'\<theta>::ev_eq) \<Rightarrow> ('\<sigma> relation) \<Rightarrow> (('\<theta>, '\<sigma>) action \<Rightarrow> ('\<theta>, '\<sigma>) action) \<Rightarrow> ('\<sigma> \<Rightarrow> '\<theta> set) \<Rightarrow> ('\<theta>, '\<sigma>) action \<Rightarrow> ('\<theta>, '\<sigma>) action" where
+"iPrefix c i j S P \<equiv> action_of(R(true \<turnstile> (\<lambda> (A, A'). (do_I c (S (more A))) (A, A') & more A' = more A)))`;` P"
+
+definition
+oPrefix::"('\<sigma> \<Rightarrow>'\<theta>) \<Rightarrow> ('\<theta>::ev_eq, '\<sigma>) action \<Rightarrow> ('\<theta>, '\<sigma>) action" where
+"oPrefix c P \<equiv> action_of(R(true \<turnstile> (do c) \<and> (\<lambda> (A, A'). more A' = more A)))`;` P"
 
 definition Prefix0::"'\<theta> \<Rightarrow> ('\<theta>::ev_eq, '\<sigma>) action \<Rightarrow> ('\<theta>, '\<sigma>) action" where
-"Prefix0 c P \<equiv> action_of(R(true \<turnstile> (do c) \<and> (\<lambda> (A, A'). more A' = more A)))`;` P"
+"Prefix0 c P \<equiv> action_of(R(true \<turnstile> (do (\<lambda> _. c)) \<and> (\<lambda> (A, A'). more A' = more A)))`;` P"
 
 definition 
 read::"('v \<Rightarrow> '\<theta>) \<Rightarrow> ('v, '\<sigma>) var_list \<Rightarrow> ('\<theta>::ev_eq, '\<sigma>) action \<Rightarrow> ('\<theta>, '\<sigma>) action"
-where  "read c x P  \<equiv> Prefix c x UNIV P"
+where  "read c x P  \<equiv> iPrefix (\<lambda> A. c (select x A)) (\<lambda> (s, s'). \<exists> a. s' = increase x a s) (Let x) (\<lambda>_. range c) P"
+
+definition 
+read1::"('v \<Rightarrow> '\<theta>) \<Rightarrow> ('v, '\<sigma>) var_list \<Rightarrow> ('\<sigma> \<Rightarrow> 'v set) \<Rightarrow> ('\<theta>::ev_eq, '\<sigma>) action \<Rightarrow> ('\<theta>, '\<sigma>) action"
+where  "read1 c x S P  \<equiv> iPrefix (\<lambda> A. c (select x A)) (\<lambda> (s, s'). \<exists> a. a\<in>(S s) & s' = increase x a s) (Let x) (\<lambda>s. c`(S s)) P"
 
 definition 
 write1::"('v \<Rightarrow> '\<theta>) \<Rightarrow> ('\<sigma> \<Rightarrow> 'v) \<Rightarrow> ('\<theta>::ev_eq, '\<sigma>) action \<Rightarrow> ('\<theta>, '\<sigma>) action"
-where "write1 c a P \<equiv> Prefix c (\<lambda> s. [a s], (\<lambda> x. \<lambda>y. y)) UNIV P"
+where "write1 c a P \<equiv> oPrefix (\<lambda> A. c (a A)) P"
 
 definition 
 write0::"'\<theta> \<Rightarrow> ('\<theta>::ev_eq, '\<sigma>) action \<Rightarrow> ('\<theta>, '\<sigma>) action" 
@@ -453,84 +905,116 @@ where "write0 c P \<equiv> Prefix0 c P"
 syntax
 "_read"  ::"[id, pttrn, ('\<theta>, '\<sigma>) action] => ('\<theta>, '\<sigma>) action" ("(_`?`_ /\<rightarrow> _)")
 "_readS" ::"[id, pttrn, '\<theta> set,('\<theta>, '\<sigma>) action] => ('\<theta>, '\<sigma>) action" ("(_`?`_`:`_ /\<rightarrow> _)")
+"_readSS" ::"[id, pttrn, '\<sigma> => '\<theta> set,('\<theta>, '\<sigma>) action] => ('\<theta>, '\<sigma>) action" ("(_`?`_`\<in>`_ /\<rightarrow> _)")
 "_write" ::"[id, '\<sigma>, ('\<theta>, '\<sigma>) action] => ('\<theta>, '\<sigma>) action" ("(_`!`_ /\<rightarrow> _)")
 "_writeS"::"['\<theta>, ('\<theta>, '\<sigma>) action] => ('\<theta>, '\<sigma>) action" ("(_ /\<rightarrow> _)")
 
 translations
 "_read c p P"    == "CONST read c (VAR_LIST p) P" 
-"_readS c p b P" == "CONST Prefix c (VAR_LIST p) b P"
-"_write c p P"   == "CONST write1 c p P"  
+"_readS c p b P" == "CONST read1 c (VAR_LIST p) (\<lambda>_. b) P"
+"_readSS c p b P" == "CONST read1 c (VAR_LIST p) b P"
+"_write c p P"   == "CONST write1 c p P"
 "_writeS a P"    == "CONST write0 a P"
 
 lemma Prefix_is_action:
-"(R(true \<turnstile> (do_I c x S) \<and> (\<lambda> (A, A'). more A' = more A))) : action"
-by (auto simp add: action_def intro: rd_is_CSP)
+"(R(true \<turnstile> (do c) \<and> (\<lambda> (A, A'). more A' = more A))) \<in> {p. is_CSP_process p}"
+by (auto intro: rd_is_CSP)
+
+lemma Prefix1_is_action:
+"(R(true \<turnstile> \<lambda>(A, A'). do_I c (S (alpha_rp.more A)) (A, A') \<and> alpha_rp.more A' = alpha_rp.more A)) \<in> {p. is_CSP_process p}"
+by (auto intro: rd_is_CSP)
 
 lemma Prefix0_is_action:
-"(R(true \<turnstile> (do c) \<and> (\<lambda> (A, A'). more A' = more A))) : action"
-by (auto simp add: action_def intro: rd_is_CSP)
+"(R(true \<turnstile> (do c) \<and> (\<lambda> (A, A'). more A' = more A))) \<in> {p. is_CSP_process p}"
+by (auto intro: rd_is_CSP)
 
-lemmas Prefix_is_CSP = Prefix_is_action[simplified action_def]
+lemmas Prefix_is_CSP = Prefix_is_action[simplified]
 
-lemmas Prefix0_is_CSP = Prefix0_is_action[simplified action_def]
+lemmas Prefix1_is_CSP = Prefix1_is_action[simplified]
 
-lemma relation_of_Prefix:
-"relation_of (Prefix c x S P) = 
-((R(true \<turnstile> (do_I c x S) \<and> (\<lambda> (A, A'). more A' = more A)));; relation_of P)"
-by (simp add: Prefix_def relation_of_Seq action_of_inverse Prefix_is_action)
+lemmas Prefix0_is_CSP = Prefix0_is_action[simplified]
+
+lemma relation_of_iPrefix:
+"relation_of (iPrefix c i j S P) = 
+((R(true \<turnstile> (\<lambda> (A, A'). (do_I c (S (more A))) (A, A') & more A' = more A)));; relation_of P)"
+by (simp add: iPrefix_def relation_of_Seq action_of_inverse Prefix1_is_CSP)
+
+lemma relation_of_oPrefix:
+"relation_of (oPrefix c P) = 
+((R(true \<turnstile> (do c) \<and> (\<lambda> (A, A'). more A' = more A)));; relation_of P)"
+by (simp add: oPrefix_def relation_of_Seq action_of_inverse Prefix_is_CSP)
+
 
 lemma relation_of_Prefix0:
 "relation_of (Prefix0 c P) = 
-((R(true \<turnstile> (do c) \<and> (\<lambda> (A, A'). more A' = more A)));; relation_of P)"
-by (simp add: Prefix0_def relation_of_Seq action_of_inverse Prefix0_is_action)
+((R(true \<turnstile> (do (\<lambda> _. c)) \<and> (\<lambda> (A, A'). more A' = more A)));; relation_of P)"
+by (simp add: Prefix0_def relation_of_Seq action_of_inverse Prefix0_is_CSP)
 
-lemma mono_Prefix : "mono (Prefix c x s)"
-by (auto simp: mono_def less_eq_action ref_def relation_of_Prefix)
+lemma mono_iPrefix : "mono (iPrefix c i j s)"
+by (auto simp: mono_def less_eq_action ref_def relation_of_iPrefix)
+
+lemma mono_oPrefix : "mono (oPrefix c)"
+by (auto simp: mono_def less_eq_action ref_def relation_of_oPrefix)
 
 lemma mono_Prefix0 : "mono(Prefix0 c)"
 by (auto simp: mono_def less_eq_action ref_def relation_of_Prefix0)
 
-subsubsection {* Hiding *}
+subsection {* Hiding *}
 
 definition Hide::"('\<theta>::ev_eq, '\<sigma>) action \<Rightarrow> '\<theta> set \<Rightarrow> ('\<theta>, '\<sigma>) action" (infixl "\\" 18) where
-"P \\ cs \<equiv> action_of(R(\<lambda>(S, S'). \<exists> s. (diff_tr S' S) = (tr_filter (s - (tr S)) cs) \<longrightarrow>
+"P \\ cs \<equiv> action_of(R(\<lambda>(S, S'). \<exists> s. (diff_tr S' S) = (tr_filter (s - (tr S)) cs) &
              (relation_of P)(S, S'\<lparr>tr := s, ref := (ref S') \<union> cs \<rparr>));; (relation_of Skip))"
 
-(* Definition of Hide modified : to check in the semantics with Ana and Jim, *)
-(* who use a slightly stronger definition (which is unlikely to be invariant) *)
 
-lemma Hide_is_not_CSP: 
-"is_CSP_process (R(\<lambda>(S, S'). \<exists> s. (diff_tr S' S) = (tr_filter (s - (tr S)) cs) \<and> 
-        (relation_of P)(S, S'\<lparr>tr := s, ref := (ref S') \<union> cs \<rparr>)) ;; (relation_of Skip))"
-apply (rule seq_CSP)
-prefer 3
+definition 
+"hid P cs == (R(\<lambda>(S, S'). \<exists> s. (diff_tr S' S) = (tr_filter (s - (tr S)) cs) & (relation_of P)(S, S'\<lparr>tr := s, ref := (ref S') \<union> cs \<rparr>)) ;; (relation_of Skip))"
+
+lemma hid_is_R: "hid P cs is R healthy"
+apply (simp add: hid_def)
+apply (rule seq_R)
+apply (simp add: Healthy_def R_idem2)
+apply (rule CSP_is_R)
 apply (rule relation_of_CSP)
-apply (auto simp: csp_defs rp_defs design_defs diff_tr_def prefix_def fun_eq_iff split: cond_splits)
-apply (subst CSP_is_rd, auto simp: rp_defs relation_of_CSP design_defs fun_eq_iff split: cond_splits)
-oops
-
-lemma Hide_is_action: 
-"(R(\<lambda>(S, S'). \<exists> s. (diff_tr S' S) = (tr_filter (s - (tr S)) cs) \<longrightarrow>
-   (relation_of P)(S, S'\<lparr>tr := s, ref := (ref S') \<union> cs \<rparr>));; (relation_of Skip)) : action"
-  apply (simp add: action_def)
-  apply (rule seq_CSP)
-  prefer 3
-  apply (rule relation_of_CSP)
-  apply (simp add: rp_defs design_defs fun_eq_iff csp_defs, auto split: cond_splits)
-  apply (subst CSP_is_rd, auto simp: rp_defs relation_of_CSP design_defs fun_eq_iff split: cond_splits)
 done
 
-lemmas Hide_is_CSP = Hide_is_action[simplified action_def]
+lemma hid_Skip: "hid P cs = (hid P cs ;; relation_of Skip)"
+by (simp add: hid_def comp_assoc[symmetric] Skip_comp_absorb)
+
+lemma hid_is_CSP1: "hid P cs is CSP1 healthy"
+apply (auto simp: design_defs CSP1_def hid_def rp_defs fun_eq_iff)
+apply (rule_tac b="a" in comp_intro)
+apply (clarsimp split: cond_splits)
+apply (subst CSP_is_rd, auto simp: rp_defs relation_of_CSP design_defs fun_eq_iff split: cond_splits)
+apply (auto simp: diff_tr_def relation_of_Skip rp_defs design_defs true_def split: cond_splits)
+apply (rule_tac x="[]" in exI, auto)
+done
+
+lemma hid_is_CSP2: "hid P cs is CSP2 healthy"
+apply (simp add: hid_def)
+apply (rule seq_CSP2)
+apply (rule CSP_is_CSP2)
+apply (rule relation_of_CSP)
+done
+
+lemma hid_is_CSP: "is_CSP_process (hid P cs)"
+by (auto simp: csp_defs hid_is_CSP1 hid_is_R hid_is_CSP2)
+
+lemma Hide_is_action: 
+"(R(\<lambda>(S, S'). \<exists> s. (diff_tr S' S) = (tr_filter (s - (tr S)) cs) &
+   (relation_of P)(S, S'\<lparr>tr := s, ref := (ref S') \<union> cs \<rparr>));; (relation_of Skip)) \<in> {p. is_CSP_process p}"
+by (simp add: hid_is_CSP[simplified hid_def])
+
+lemmas Hide_is_CSP = Hide_is_action[simplified]
 
 lemma relation_of_Hide:
 "relation_of (P \\ cs) = (R(\<lambda>(S, S'). \<exists> s. (diff_tr S' S) = (tr_filter (s - (tr S)) cs)
-        \<longrightarrow> (relation_of P)(S, S'\<lparr>tr :=s, ref := (ref S') \<union> cs \<rparr>));; (relation_of Skip))"
-  by (simp add: Hide_def action_of_inverse Hide_is_action)
+        & (relation_of P)(S, S'\<lparr>tr :=s, ref := (ref S') \<union> cs \<rparr>));; (relation_of Skip))"
+  by (simp add: Hide_def action_of_inverse Hide_is_CSP)
 
 lemma mono_Hide : "mono(\<lambda> P. P \\ cs)"
-by (auto simp: mono_def less_eq_action ref_def prefix_def utp_defs relation_of_Hide rp_defs)
+by (auto simp: mono_def less_eq_action ref_def prefixeq_def utp_defs relation_of_Hide rp_defs)
 
-subsubsection {* Recursion \label{subsec:Recursion}*}
+subsection {* Recursion *}
 
 text {* To represent the recursion operator "@{text \<mu>}" over actions, we use the
 universal least fix-point operator "@{const lfp}" defined in the HOL library for lattices. 
@@ -569,5 +1053,6 @@ apply (subst lfp_unfold)
 apply (auto simp: A B)
 done 
 
+term Nat.Suc
 (*>*)
 end
