thys/Circus/Refinement.thy
@@ -1,60 +1,11 @@
-(*  Title:       Isabelle/Circus
-    Author:      Abderrahmane Feliachi, Burkhart Wolff, Marie-Claude Gaudel
-                 Univ. Paris-Sud / LRI
-    Maintainer:  Abderrahmane Feliachi
-*)
-
-header {* Using Isabelle/\Circus\ for Refinement Proofs
-          \label{Refinement} \label{Section:framework}*}
+header {* Refinement and Simulation *}
 
 theory Refinement
-imports Denotational_Semantics
+imports Denotational_Semantics Circus_Syntax 
 begin
 
-subsection {* Relational and Functional Refinement in \Circus *}
 
-text{*
-
-The main goal of Isabelle/\Circus\ is to provide a proof environment for \Circus\ processes. 
-The ``shallow-embedding'' of \Circus\ and UTP in Isabelle/HOL offers the 
-possibility to reuse proof procedures, infrastructure and theorem libraries already 
-existing in Isabelle/HOL. In this chapter, we will demonstrate 
-Isabelle/\Circus\ 's potential by one of the
-potential application areas, namely refinement proofs between processes
-(the other important line of interest is the automated generation of
-test-cases, which we adress in the future). 
-
-In order to enter Isabelle/\Circus specifications, an own parser has
-been developed (the the interested reader is referred to: 
-@{url "http://www.lri.fr/~feliachi/IsabelleCircus/"}). In the
-following, we will present our example both in high-level syntax
-implementing common textbook notation on \Circus\ as well as the
-semantic code resulting from these expressions in the context of 
-the denotational semantics theories.
- 
-The Isabelle/\Circus\ parser (not discussed here), provides a means
-to encode a process specification in terms of the presented
-semantic theories, such that proofs of, e. g., refinement properties 
-can be developped using the ISAR language for structured proofs.
-
-In the following, 
-we provide a small example of action refinement proof. 
-The refinement relation is defined as the universal reverse implication in the UTP. 
-In \Circus ,it is defined as follows: 
-
-\begin{isar}
-definition A1 \<sqsubseteq>c A2 \<equiv>  (Rep_Action A1) \<sqsubseteq>utp (Rep_Action A2)
-\end{isar}
-where A1 and A2 are \Circus\ actions, \inlineisar+\<sqsubseteq>c+ and \inlineisar+\<sqsubseteq>utp+ stands 
-respectively for refinement relation on \Circus\ actions and on UTP predicate.
-
-This definition assumes that the actions A1 and A2 share the same alphabet (binding) 
-and the same channels. In general, refinement involves an important data evolution and growth. 
-The data refinement is defined in \cite{SWC02,CSW03} by backwards and forwards simulations. 
-In this paper, we restrict ourselves to a special case, the so-called \emph{functional} 
-backwards simulation. This refers to the fact that the abstraction relation 
-@{term R} that relates concrete and abstract actions is just a function.
-*}
+subsection {* Definitions *}
 
 text {* In the following, data (state) simulation and functional backwards simulation
  are defined. The simulation is defined as a function $S$, that corresponds to a state 
@@ -63,70 +14,16 @@ text {* In the following, data (state) simulation and functional backwards simul
 definition "Simul S b = extend (make (ok b) (wait b) (tr b) (ref b)) (S (more b))"
 
 definition 
-Simulation::"('\<theta>::ev_eq,'\<sigma>) action \<Rightarrow> ('\<sigma>\<^sub>1 \<Rightarrow> '\<sigma>) \<Rightarrow> ('\<theta>, '\<sigma>\<^sub>1) action \<Rightarrow> bool" ("_ \<preceq>_ _") 
+Simulation::"('\<theta>::ev_eq,'\<sigma>) action \<Rightarrow> ('\<sigma>1 \<Rightarrow> '\<sigma>) \<Rightarrow> ('\<theta>, '\<sigma>1) action \<Rightarrow> bool" ("_ \<preceq>_ _") 
 where
 "A \<preceq>S B \<equiv> \<forall> a b. (relation_of B) (a, b) \<longrightarrow> (relation_of A) (Simul S a, Simul S b)"
 
-text {*
-\subsection{Refinement Proofs}
+subsection {* Proofs *}
 
-This definition can be used to transform the proof of refinement to a simple 
-proof of implication by unfolding the operators using their underlying relational semantics. 
-The problem with this approach is the proof size explodes. 
-In order to avoid this, general refinement laws have been proposed in \cite{CSW03} to deal 
-with the refinement of \Circus\ actions at operators level and not at UTP level. We re-introduced 
-and proved a subset of theses laws in our environment (see Table \ref{table:laws}), i.e.
-we \emph{derived} them from the definitions of the \Circus\ operators in the denotational
-semantics. 
-
-\setlength{\tabcolsep}{9pt}
-\begin{table}[h]
-\begin{center}{\footnotesize
-\begin{tabular}[t]{| c c c |}
-\hline
-& & \\
-\vspace{- 0.7 cm}
-& & \\
-\infer[\text{Seq-Sim}] {P ; P' \preceq_S Q ; Q'}{P \preceq_S Q & \quad P' \preceq_S Q'} & \multicolumn{2}{c |}{\infer[\text{Guard-Sim}] {g_1 \& P \preceq_S g_2 \& Q}{P \preceq_S Q & \quad g_1 \simeq_S g_2}} \\
-& & \\
-\vspace{- 0.55 cm}
-& & \\
-\infer[\text{Var-Sim}] {var~x \bullet P \preceq_S var~ y \bullet Q}{P \preceq_S Q & \quad x \sim_S y} & \multicolumn{2}{c |}{\infer[\text{Read-Sim}] {c?x \rightarrow P \preceq_S c?y \rightarrow Q}{P \preceq_S Q & \quad x \sim_S y}} \\
-& & \\
-\vspace{- 0.55 cm}
-& & \\
-\infer[\text{Ndet-Sim}] {P \sqcap P' \preceq_S Q \sqcap Q'}{P \preceq_S Q & \quad P' \preceq_S Q'} & \multicolumn{2}{c |}{\infer[\text{Write-Sim}] {c!x \rightarrow P \preceq_S c!y \rightarrow Q}{P \preceq_S Q & \quad x \sim_S y}} \\
-& & \\
-\vspace{- 0.55 cm}
-& & \\
-\infer[\text{Mu-Sim}] {\mu X \bullet P~X \preceq_S \mu Y \bullet Q~Y}{\infer*{P~X \preceq_S Q~Y}{[X \preceq_S Y]} & mono~P & mono~Q} & \multicolumn{2}{c |}{\infer[\text{Det-Sim}] {P \Box P' \preceq_S Q \Box Q'}{P \preceq_S Q & \quad P' \preceq_S Q'}} \\
-& & \\
-\vspace{- 0.55 cm}
-& & \\
-\infer[\text{Sch-Sim}] {schema~sc_1 \preceq_S schema~sc_2}{\infer*{Pre~sc_2~A}{[Pre~sc_1~(S~A)]} & \infer*{sc_1~(S~A, S~A')}{[Pre~sc_1~(S~A) & sc_2~(A, A')]}} & \multicolumn{2}{c |}{\infer[\text{Sync-Sim}] {a \rightarrow P \preceq_S a \rightarrow Q}{P \preceq_S Q}} \\
-& & \\
-\vspace{- 0.55 cm}
-& & \\
-\multicolumn{2}{| c}{\infer[\text{Par-Sim}] {P \llbracket ns_1 | cs | ns_2 \rrbracket P' \preceq_S Q \llbracket ns'_1 | cs | ns'_2 \rrbracket Q'}{P \preceq_S Q & P' \preceq_S Q' & ns_1 \sim_S ns'_1 & ns_2 \sim_S ns'_2}} &
-\infer[\text{Skip-Sim}] {Skip \preceq_S Skip}{} \\
-& & \\
-\hline
-\end{tabular}
-  \caption{\label{table:laws} Proved refinement laws}}
-\end{center}
-\end{table}
-
-
-In Table \ref{table:laws}, the relations ``$x \sim_S y$'' and ``$g_1 \simeq_S g_2$'' 
-record the fact that the variable $x$ (repectively the guard $g_1$) is refined by 
-the variable $y$ (repectively by the guard $g_2$) w.r.t the simulation function $S$.
-
-These laws can be used in complex refinement proofs to simplify them at the \Circus\ level. 
-More rules can be defined and proved to deal with more complicated statements like combination 
-of operators for example. Using these laws, and exploiting the advantages of a shallow embedding, 
-the automated proof of refinement becomes surprisingly simple.
-The proofs of these laws are given in the following:
-*}
+text {* In order to simplify refinement proofs, some general refinement laws are 
+defined to deal with the refinement of Circus actions at operators level and not at UTP level. 
+Using these laws, and exploiting the advantages of a shallow embedding, the automated proof of
+refinement becomes surprisingly simple. *}
 
 lemma Stop_Sim: "Stop \<preceq>S Stop"
 by (auto simp: Simulation_def relation_of_Stop rp_defs design_defs Simul_def alpha_rp.defs 
@@ -153,18 +50,54 @@ by (auto simp: Simulation_def relation_of_Det design_def rp_defs Simul_def alpha
          dest: A[simplified Simulation_def Simul_def, rule_format]
                B[simplified Simulation_def Simul_def, rule_format])
 
-lemma Sch_Sim:
+lemma Schema_Sim:
   assumes A: "\<And> a. (Pre sc1) (S a) \<Longrightarrow> (Pre sc2) a"
   and B: "\<And> a b. \<lbrakk>Pre sc1 (S a) ; sc2 (a, b)\<rbrakk> \<Longrightarrow> sc1 (S a, S b)"
   shows "(Schema sc1) \<preceq>S (Schema sc2)"
 by (auto simp: Simulation_def Simul_def relation_of_Schema rp_defs design_defs alpha_rp.defs A B
          split: cond_splits)
 
+lemma SUb_Sim:
+  assumes A: "\<And> a. (Pre sc1) (S a) \<Longrightarrow> (Pre sc2) a"
+  and B: "\<And> a b. \<lbrakk>Pre sc1 (S a) ; sc2 (a, b)\<rbrakk> \<Longrightarrow> sc1 (S a, S b)"
+  and C: "P \<preceq>S Q"
+  shows "(state_update_before sc1 P) \<preceq>S (state_update_before sc2 Q)"
+apply (auto simp: Simulation_def Simul_def relation_of_state_update_before rp_defs design_defs alpha_rp.defs A B
+         split: cond_splits)
+apply (drule C[simplified Simulation_def, rule_format])
+apply (rule_tac b="Simul S ba" in comp_intro)
+apply (auto simp: A B Simul_def alpha_rp.defs)
+apply (clarsimp split: cond_splits)+
+apply (drule C[simplified Simulation_def, rule_format])
+apply (rule_tac b="Simul S ba" in comp_intro)
+apply (auto simp: A B Simul_def alpha_rp.defs)
+apply (clarsimp split: cond_splits)+
+apply (case_tac "ok aa", simp_all)
+apply (erule notE) back
+apply (drule C[simplified Simulation_def, rule_format])
+apply (rule_tac b="Simul S ba" in comp_intro)
+apply (auto simp: A B Simul_def alpha_rp.defs)
+apply (clarsimp split: cond_splits)+
+apply (rule A)
+apply (case_tac "Pre sc1 (S (alpha_rp.more aa))", simp_all)
+apply (erule notE) back
+apply (drule C[simplified Simulation_def, rule_format])
+apply (rule_tac b="Simul S ba" in comp_intro)
+apply (auto simp: A B Simul_def alpha_rp.defs)
+apply (clarsimp split: cond_splits)+
+apply (drule C[simplified Simulation_def, rule_format])
+apply (rule_tac b="Simul S ba" in comp_intro)
+apply (auto simp: A B Simul_def alpha_rp.defs)
+apply (clarsimp split: cond_splits)+
+apply (rule B, auto)
+done
+
 lemma Seq_Sim:
   assumes A: "P \<preceq>S Q" and B: "P' \<preceq>S Q'"
   shows "(P `;` P') \<preceq>S (Q `;` Q')"
 by (auto simp: Simulation_def relation_of_Seq dest: A[simplified Simulation_def, rule_format]
                                                     B[simplified Simulation_def, rule_format])
+
 
 lemma Par_Sim:
   assumes A: " P  \<preceq>S Q" and B: " P' \<preceq>S Q'"
@@ -202,7 +135,7 @@ lemma Par_Sim:
               split: cond_splits)
   apply (rule_tac b="Simul S ba" in comp_intro)
   apply (auto simp add: M_par_def alpha_rp.defs diff_tr_def fun_eq_iff ParMerge_def Simul_def
-            split : cond_splits) 
+            split : cond_splits)
   apply (rule_tac b="\<lparr>ok = ok bb, wait = wait bb, tr = tr bb, ref = ref bb, 
               \<dots> = S (alpha_rp.more bb)\<rparr>" in comp_intro, auto)
   apply (subst D[where a="(alpha_rp.more s1)" and b="(alpha_rp.more aa)", symmetric], simp)
@@ -237,12 +170,12 @@ lemma Var_Sim:
   apply (erule disjE, rule disjI1, simp, rule disjI2, simp)
   apply (simp_all add: alpha_rp.defs true_def)
   apply (rule impI, (erule conjE | simp)+)
-  apply (erule alpha_rp_eqE, simp add: B)
+  apply (simp add: B)
   apply (split cond_splits)+
   apply (simp add: alpha_rp.defs)
   apply (erule disjE, rule disjI1, simp, rule disjI2, simp_all)
   apply (rule impI, (erule conjE | simp)+)
-  apply (erule alpha_rp_eqE, simp add: B)
+  apply (simp add: B)
 done
 
 lemma Guard_Sim:
@@ -256,7 +189,7 @@ apply (auto simp: true_Guard1 false_Guard1 Simul_def alpha_rp.defs Simulation_de
             dest!: A[simplified, rule_format] Stop_Sim[simplified, rule_format])
 done
 
-lemma Sync_Sim:
+lemma Write0_Sim:
   assumes A: "P \<preceq>S Q"
   shows "a \<rightarrow> P \<preceq>S a \<rightarrow> Q "
   using   A
@@ -270,21 +203,41 @@ done
 lemma Read_Sim:
   assumes A: " P \<preceq>S Q" and B: "\<And> A. (d A) = c (S A)"
   shows "a`?`c \<rightarrow> P \<preceq>S a`?`d \<rightarrow> Q"
-  using   A
-  apply (auto simp: Simulation_def read_def relation_of_Prefix design_defs rp_defs)
+  using A
+  apply (auto simp: Simulation_def read_def relation_of_iPrefix design_defs rp_defs)
   apply (erule_tac x="ba" in allE, erule_tac x="ca" in allE, simp)
   apply (rule_tac b="Simul S ba" in comp_intro)
   apply (auto split: cond_splits simp: Simul_def alpha_rp.defs do_I_def select_def B)
+done
+
+lemma Read1_Sim:
+  assumes A: " P \<preceq>S Q" and B: "\<And> A. (d A) = c (S A)"
+  shows "a`?`c`:`s \<rightarrow> P \<preceq>S a`?`d`:`s \<rightarrow> Q"
+  using A
+  apply (auto simp: Simulation_def read1_def relation_of_iPrefix design_defs rp_defs)
+  apply (erule_tac x="ba" in allE, erule_tac x="ca" in allE, simp)
+  apply (rule_tac b="Simul S ba" in comp_intro)
+  apply (auto split: cond_splits simp: Simul_def alpha_rp.defs do_I_def select_def B)
+done
+
+lemma Read1S_Sim:
+  assumes A: " P \<preceq>S Q" and B: "\<And> A. (d A) = c (S A)" and C: "\<And> A. (s' A) = s (S A)"
+  shows "a`?`c`\<in>`s \<rightarrow> P \<preceq>S a`?`d`\<in>`s' \<rightarrow> Q"
+  using A
+  apply (auto simp: Simulation_def read1_def relation_of_iPrefix design_defs rp_defs)
+  apply (erule_tac x="ba" in allE, erule_tac x="ca" in allE, simp)
+  apply (rule_tac b="Simul S ba" in comp_intro)
+  apply (auto split: cond_splits simp: Simul_def alpha_rp.defs do_I_def select_def B C)
 done
 
 lemma Write_Sim:
   assumes A: "P \<preceq>S Q" and B: "\<And> A. (d A) = c (S A)"
   shows "a`!`c \<rightarrow> P \<preceq>S a`!`d \<rightarrow> Q "
   using A
-  apply (auto simp: Simulation_def write1_def relation_of_Prefix design_defs rp_defs)
+  apply (auto simp: Simulation_def write1_def relation_of_oPrefix design_defs rp_defs)
   apply (erule_tac x="ba" in allE, erule_tac x="ca" in allE, simp)
   apply (rule_tac b="Simul S ba" in comp_intro)
-  apply (auto split: cond_splits simp: Simul_def alpha_rp.defs do_I_def select_def B)
+  apply (auto split: cond_splits simp: Simul_def alpha_rp.defs do_def select_def B)
 done
 
 lemma Hide_Sim:
@@ -317,5 +270,52 @@ done
 
 lemma bot_Sim: "bot \<preceq>S bot"
 by (auto simp: Simulation_def rp_defs Simul_def relation_of_bot alpha_rp.defs split: cond_splits)
+
+lemma sim_is_ref: "P \<sqsubseteq> Q = P \<preceq>(id) Q"
+apply (auto simp: ref_def Simulation_def Simul_def alpha_rp.defs)
+apply (erule_tac x=a in allE)
+apply (erule_tac x=b in allE, auto)
+apply (rule_tac t="\<lparr>ok = ok a, wait = wait a, tr = tr a, ref = ref a, \<dots> = alpha_rp.more a\<rparr>" and s=a in subst, simp)
+apply (rule_tac t="\<lparr>ok = ok b, wait = wait b, tr = tr b, ref = ref b, \<dots> = alpha_rp.more b\<rparr>" and s=b in subst, simp_all)
+apply (erule_tac x=a in allE)
+apply (erule_tac x=b in allE, auto)
+apply (rule_tac s="\<lparr>ok = ok a, wait = wait a, tr = tr a, ref = ref a, \<dots> = alpha_rp.more a\<rparr>" and t=a in subst, simp)
+apply (rule_tac s="\<lparr>ok = ok b, wait = wait b, tr = tr b, ref = ref b, \<dots> = alpha_rp.more b\<rparr>" and t=b in subst, simp_all)
+done
+
+lemma ref_eq: "((P::('a::ev_eq,'b) action) = Q) = (P \<sqsubseteq> Q & Q \<sqsubseteq> P)"
+apply (rule)
+apply (simp add: ref_def)
+apply (auto simp add: ref_def fun_eq_iff relation_of_inject[symmetric])
+done
+
+lemma rd_ref: 
+assumes A:"R (P \<turnstile> Q) \<in> {p. is_CSP_process p}"
+and B:"R (P' \<turnstile> Q') \<in> {p. is_CSP_process p}"
+and C:"\<And> a b. P (a, b) \<Longrightarrow> P' (a, b)"
+and D:"\<And> a b. Q' (a, b) \<Longrightarrow> Q (a, b)"
+shows "(action_of (R (P \<turnstile> Q))) \<sqsubseteq> (action_of (R (P' \<turnstile> Q')))"
+apply (auto simp: ref_def)
+apply (subst (asm) action_of_inverse, simp add: B[simplified])
+apply (subst action_of_inverse, simp add: A[simplified])
+apply (auto simp: rp_defs design_defs C D split: cond_splits)
+done
+
+
+lemma rd_impl: 
+assumes A:"R (P \<turnstile> Q) \<in> {p. is_CSP_process p}"
+and B:"R (P' \<turnstile> Q') \<in> {p. is_CSP_process p}"
+and C:"\<And> a b. P (a, b) \<Longrightarrow> P' (a, b)"
+and D:"\<And> a b. Q' (a, b) \<Longrightarrow> Q (a, b)"
+shows "R (P' \<turnstile> Q') (a, b) \<longrightarrow> R (P \<turnstile> Q) (a::('a::ev_eq, 'b) alpha_rp_scheme, b)"
+apply (insert rd_ref[of P Q P' Q', OF A B C D])
+apply (auto simp: ref_def)
+apply (atomize, auto)
+apply (subst (asm) action_of_inverse, simp add: B[simplified])
+apply (subst (asm) action_of_inverse, simp add: A[simplified])
+apply (erule_tac x=a in allE)
+apply (erule_tac x=b in allE)
+apply (auto)
+done
 
 end
