thys/Circus/Var.thy
@@ -1,0 +1,27 @@
+header {* UTP variables *}
+
+theory Var
+imports Commands
+begin
+
+text {* UTP variables are characterized by two functions, $select$ and $update$. 
+        The variable type is then defined as a tuple ($select$ * $update$). *}
+
+type_synonym ('a, 'r) var = "('r \<Rightarrow> 'a) * (('a \<Rightarrow> 'a) \<Rightarrow> 'r \<Rightarrow> 'r)"
+
+text {* The $lookup$ function returns the corrsponding $select$ function of a variable. *}
+
+definition lookup :: "('a, 'r) var \<Rightarrow> 'r \<Rightarrow> 'a"
+  where "lookup f \<equiv> (fst f)"
+
+text {* The $assign$ function uses the $update$ function of a variable to update its value.*}
+
+definition assign :: "('a, 'r) var \<Rightarrow> 'a \<Rightarrow> 'r \<Rightarrow> 'r"
+  where "assign f v \<equiv> (snd f) (\<lambda> _ . v)"
+
+text {* The $VAR$ function allows to retrieve a variable given its name.*}
+
+syntax "_VAR" :: "id \<Rightarrow> ('a, 'r) var"  ("VAR _")
+translations "VAR x" => "(x, _update_name x)"
+
+end
